core/RegAlloc.v
@@ -1,32 +1,33 @@
 From Ssara.Core Require Import Syntax.
+From Ssara.Core Require Import RegClass.
 From Ssara.Core Require Import Utils.
 From Ssara.Core Require Import InterfGraph.
-From Stdlib Require Import Lists.List.
+From Ssara.Core Require Import Dict.
 From Stdlib Require Import ZArith.
+From Stdlib Require Import Lists.List.
 Import ListNotations.
 From Stdlib Require Import Bool.
+From Stdlib Require Import ListSet.
 
 (* Check whether regs are neighbors of r *)
-Definition neighbors (r : reg) (regs : list reg) (g : ig) : bool :=
-  regs_mem r (ig_v g) &&
+Definition neighborsb (r : reg) (regs : list reg) (g : ig) : bool :=
+  vregs_mem r (dict_keys g) &&
   fold_left
     (fun b r' =>
-      b && (
-        (r =? r') ||
-        regs_mem r' (ig_nbors g r)
-      )
-    )
+      b &&
+      ((r =? r') ||
+        vregs_mem r' (dict_map g r)))
     regs
     true
 .
 
-Definition simplicial (r : reg) (g : ig) : bool :=
-  let regs := ig_nbors g r in
-  regs_mem r (ig_v g) &&
+Definition simplicialb (r : reg) (g : ig) : bool :=
+  let regs := dict_map g r in
+  vregs_mem r (dict_keys g) &&
   fold_left (* Check whether the neighbor set of r is a clique *)
     (fun b r =>
       b &&
-      neighbors r regs g
+      neighborsb r regs g
     )
     regs
     true
@@ -37,10 +38,10 @@ Definition find_next (g : ig) : option reg :=
     match regs with
     | nil => None
     | r :: rs =>
-      if simplicial r g then Some r else find_next_aux rs
+      if simplicialb r g then Some r else find_next_aux rs
     end
   in
-  find_next_aux (ig_v g)
+  find_next_aux (dict_keys g)
 .
 
 Fixpoint eliminate (g : ig) (fuel : nat) : ig * list reg :=
@@ -56,6 +57,65 @@ Fixpoint eliminate (g : ig) (fuel : nat) : ig * list reg :=
     end
   end
 .
+
+From Ssara.Core Require Import RegPregInstance.
+From Ssara.Core Require Import RegVregInstance.
+
+Instance dict_coloring_instance : DictClass := {|
+  key := vreg;
+  value := preg;
+  default := NOREG;
+  key_eq_dec := Nat.eq_dec;
+|}.
+Definition coloring := dict.
+
+(*
+  The partial_coloring is performed this way:
+  - Get a perfect elimination order (ordering that eliminates simplicial nodes first)
+  - For each node in the peo reinsert it into the graph and color it differently wrt its neighbor
+*)
+Definition color_diff (colors : list preg) : option preg :=
+  match set_diff preg_eq_dec preg_all colors with
+  | nil => None
+  | c :: _ => Some c
+  end
+.
+
+(*
+  By definition of peo the `nbors` list contains all the neighbors of `v`
+*)
+Definition color_vreg (v : vreg) (deleted : list vreg) (c : coloring) (g : ig) : option preg :=
+  let nbors := dict_map g v in
+  let colors := map (dict_map c) nbors in
+  color_diff colors
+.
+
+Definition color (peo : list vreg) (g : ig) : option coloring :=
+  let fix color_aux (peo : list vreg) (deleted : list vreg) (c : coloring) (g : ig) : option coloring :=
+    match peo with
+    | nil => Some c
+    | v :: peo' =>
+      match color_vreg v deleted c g with
+      | Some p =>
+        let c' := dict_update c v p in
+        color_aux peo' (v :: deleted) c' g
+      | None => None
+      end
+    end
+  in
+  color_aux peo nil dict_empty g
+.
+
+(* Definition vphi := phi reg_vreg_instance.
+Definition pphi := phi reg_preg_instance.
+
+Definition color_phi (p : phi) (c : coloring) :=
+  match p with
+  | Phi v vs => Phi (dict_map c v) (fold_left (dict_map c) vs)
+  end
+.
+
+Definition color_program (p : program) (c : coloring) : program :=
 
 Module Example1.
   CoFixpoint example_block_2 : block :=
@@ -96,20 +156,26 @@ Module Example1.
 
   Compute
     let g := get_ig example_block_1 fuel in
-    map (fun r => (r, ig_nbors g r)) (ig_v g)
+    dict_list g
   .
 
   Compute
     let g := get_ig example_block_1 fuel in
-    let (g' , l) := eliminate g fuel in
-    l
-    (* map (fun r => (r, (ig_nbors g) r)) (ig_v g) *)
+    let (g' , peo) := eliminate g fuel in
+    peo
+  .
+
+  Compute
+    let g := get_ig example_block_1 fuel in
+    let (g' , peo) := eliminate g fuel in
+    let c := color peo g in
+    dict_list c
   .
 End Example1.
 
 (*
 TODO:
+- Generic map data type V
 - Register allocation
-- Generic map data type
 - Maybe visualize the interference graph in OCaml
-*)
+*) *)
