core/Utils.v
@@ -1,45 +1,37 @@
 From Ssara.Core Require Import Syntax.
+From Ssara.Core Require Import RegClass.
 From Ssara.Core Require Import Vm.
 From Stdlib Require Import ZArith.
 From Stdlib Require Import ListSet.
 From Stdlib Require Import Lists.List.
 
-From Ssara.Core Require Import RegNatInstance.
-Existing Instance reg_instance.
+From Ssara.Core Require Import RegVregInstance.
+Existing Instance reg_vreg_instance.
 
-(* Set of registers *)
-Definition reg_eq_dec : forall r r' : reg, {r = r'} + {r <> r'} := reg_eq_dec.
-Definition regs_union := set_union reg_eq_dec.
-Definition regs_diff := set_diff reg_eq_dec.
-Definition regs_add := set_add reg_eq_dec.
-Definition regs_remove := set_remove reg_eq_dec.
-
-(* Lemma regs_remove_absence :
-  forall (r : reg) (regs : set reg),
-    In r regs -> length (regs_remove r regs) < length regs
-.
-Proof.
-  induction regs as [| x xs IH]; simpl; intros Hin.
-  - inversion Hin.
-  - destruct reg_eq_dec as [Heq | Hneq].
-    + subst.
-      apply Nat.lt_succ_diag_r.
-    + simpl.
-      apply -> Nat.succ_lt_mono.
-      assert (In r xs) as Hin_t by (destruct Hin; [contradiction | assumption]). *)
-
-Definition regs_mem := set_mem reg_eq_dec.
-
-(* Set of labels *)
-Definition l_eq_dec : forall r r' : reg, {r = r'} + {r <> r'} := Nat.eq_dec.
-Definition ls_union := set_union l_eq_dec.
-Definition ls_diff := set_diff l_eq_dec.
-Definition ls_add := set_add l_eq_dec.
+(* Set of virtual registers *)
+Definition vreg_eq_dec : forall r r' : reg, {r = r'} + {r <> r'} := reg_eq_dec.
+Definition vregs_union := set_union reg_eq_dec.
+Definition vregs_diff := set_diff reg_eq_dec.
+Definition vregs_add := set_add reg_eq_dec.
+Definition vregs_remove := set_remove reg_eq_dec.
+Definition vregs_mem := set_mem reg_eq_dec.
 
 (* Convert option to list *)
 Definition option_to_list {A : Type} (x : option A) : list A :=
   match x with
   | Some x' => x' :: nil
   | None => nil
+  end
+.
+
+(* Convert list option to list *)
+Fixpoint list_option_to_list {A : Type} (l : list (option A)) : list A :=
+  match l with
+  | nil => nil
+  | x :: xs =>
+    match x with
+    | Some y => y :: (list_option_to_list xs)
+    | None => (list_option_to_list xs)
+    end
   end
 .
