core/Dict.v
@@ -1,0 +1,43 @@
+From Ssara.Core Require Import Syntax.
+From Ssara.Core Require Import Vm.
+From Ssara.Core Require Import Utils.
+From Stdlib Require Import Lists.List.
+From Stdlib Require Import ZArith.
+From Stdlib Require Import ListSet.
+Import ListNotations.
+
+Section Dict.
+
+Class DictClass := {
+  key : Set;
+  value : Type;
+  default : value;
+  key_eq_dec : forall k k' : key, {k = k'} + {k <> k'};
+}.
+Context {dict_instance : DictClass}.
+
+Definition dict : Type := set key * (key -> value).
+Definition dict_empty : dict := (nil, fun _ => default).
+
+Definition dict_update (d : dict) (k : key) (v : value) : dict :=
+  let (keys, m) := d in
+  (set_add key_eq_dec k keys, fun k' => if key_eq_dec k' k then v else m k')
+.
+
+Definition dict_map (d : dict) (k : key) : value :=
+  let (_, m) := d in m k
+.
+
+Definition dict_keys (d : dict) : set key :=
+  let (keys, _) := d in keys
+.
+
+Definition dict_values (d : dict) : set value :=
+  let (keys, m) := d in map m keys
+.
+
+Definition dict_list (d : dict) : list (key * value) :=
+  let (keys, m) := d in map (fun k => (k, m k)) keys
+.
+
+End Dict.
