core/RegNatInstance.v
@@ -1,8 +1,0 @@
-From Stdlib Require Import PeanoNat.
-From Ssara.Core Require Import Syntax.
-
-Instance reg_instance : RegClass := {|
-  reg := nat;
-  reg_eqb := Nat.eqb;
-  reg_eq_dec := Nat.eq_dec;
-|}.
