core/RegVregInstance.v
@@ -1,0 +1,10 @@
+From Stdlib Require Import PeanoNat.
+From Ssara.Core Require Import RegClass.
+
+Definition vreg : Set := nat.
+
+Instance reg_vreg_instance : RegClass := {|
+  reg := vreg;
+  reg_eqb := Nat.eqb;
+  reg_eq_dec := Nat.eq_dec;
+|}.
