core/RegClass.v
@@ -1,0 +1,5 @@
+Class RegClass := {
+  reg : Set;
+  reg_eqb : reg -> reg -> bool;
+  reg_eq_dec : forall r r' : reg, {r = r'} + {r <> r'};
+}.
